We replace the $f^{'}(x_k)$ in [[Newton's method]] with ::  $\frac{f(x_{k})-f(x_{0})}{x_{k}-x_{0}}$
and we can get $x_{k+1} = x_{k}-\frac{f (x_{k})}{f (x_{k})-f (x_{0})}(x_k-x_{0})$ ([pdf](zotero://open-pdf/library/items/X3UESHXG?page=74&annotation=M4EQCGPX))
# [[convergent|convergence]] rate of the method 
When $x_0$ is sufficiently close to $x^{∗}$, one has $|φ′(x∗)| < 1$ and we get **linear convergence** of the Newton’s secant method ([pdf](zotero://open-pdf/library/items/X3UESHXG?page=76&annotation=8G8MWHBI))