#ca

the [[inverse function]] of [[exponential function]]
$log_bx =y \iff b^y =x$

## calculation laws

1.$log_b(xy) =log_bx + log_by$
2.$log_b\frac{x}{y} = log_bx -log_by$
3.$log_b(x^r) = rlog_bx$

## derivatives

$\frac{d(log_bx)}{dx} = \frac{1}{xlnb}$

## Natural Logarithm

$log_ex = lnx$

### properties

$lne = 1$

### number e

for $f(1)^{'} = 1$ ,we express it as limit
$f(1)^{'} = lim_{x \to 0} \frac{ln(1+x) - ln(1)}{x} = lim_{x \to 0} ln(1+x)^{\frac{1}{x}} = 1$
therefore
$e = lim_{x \to 0}e^{ln(1+x)^{\frac{1}{x}}} = lim_{x \to 0}(1 + x)^{\frac{1}{x}} = lim_{n \to \infty}(1 + n)^n$

### derivative

$\frac{dlnx}{dx} = \frac{1}{x}$

## change of base formula

for any $b \neq 0$
$log_bx = \frac{lnx}{lnb}$
